F_mu/fundamental.v
@@ -1,0 +1,210 @@
+Require Import iris.program_logic.hoare.
+Require Import iris.program_logic.lifting.
+Require Import iris.algebra.upred_big_op.
+Require Import F_mu.lang F_mu.typing F_mu.rules F_mu.logrel.
+Require Import Vlist.
+Import uPred.
+
+Section typed_interp.
+  Context {Σ : iFunctor}.
+  Implicit Types P Q R : iProp lang Σ.
+  Notation "# v" := (of_val v) (at level 20).
+
+  Canonical Structure leibniz_val := leibnizC val.
+
+  Canonical Structure leibniz_le n m := leibnizC (n ≤ m).
+
+  Ltac ipropsimpl :=
+    repeat
+      match goal with
+      | [|- (_ ⊢ (_ ∧ _))%I] => eapply and_intro
+      | [|- (▷ _ ⊢ ▷ _)%I] => apply later_mono
+      | [|- (_ ⊢ ∃ _, _)%I] => rewrite -exist_intro
+      | [|- ((∃ _, _) ⊢ _)%I] => let v := fresh "v" in rewrite exist_elim; [|intros v]
+      end.
+
+  Local Hint Extern 1 => progress ipropsimpl.
+
+  Local Tactic Notation "smart_wp_bind" uconstr(ctx) uconstr(t) ident(v) :=
+    rewrite -(@wp_bind _ _ _ [ctx]) /= -wp_impl_l; apply and_intro; [
+    apply (@always_intro _ _ _ t), forall_intro=> v /=; apply impl_intro_l| eauto with itauto].
+
+  Local Tactic Notation "smart_wp_bind" uconstr(ctx) ident(v) :=
+    rewrite -(@wp_bind _ _ _ [ctx]) /= -wp_mono; eauto; intros v; cbn.
+
+  Create HintDb itauto.
+
+  Local Hint Extern 3 ((_ ∧ _) ⊢ _)%I => rewrite and_elim_r : itauto.
+  Local Hint Extern 3 ((_ ∧ _) ⊢ _)%I => rewrite and_elim_l : itauto.
+  Local Hint Extern 3 (_ ⊢ (_ ∨ _))%I => rewrite -or_intro_l : itauto.
+  Local Hint Extern 3 (_ ⊢ (_ ∨ _))%I => rewrite -or_intro_r : itauto.
+  Local Hint Extern 2 (_ ⊢ ▷ _)%I => etransitivity; [|rewrite -later_intro] : itauto.
+  
+  Local Ltac value_case := rewrite -wp_value/= ?to_of_val //; auto 2.
+  
+  Lemma typed_interp k Δ Γ vs e τ
+        (Htyped : typed k Γ e τ)
+        (Hctx : closed_ctx k Γ)
+        (HC : closed_type k τ)
+        (HΔ : VlistAlwaysStable Δ)
+    : length Γ = length vs →
+      Π∧ zip_with (λ τ v, interp k (` τ) (proj2_sig τ) Δ v) (closed_ctx_list _ Γ Hctx) vs ⊢
+                  WP (e.[env_subst vs]) @ ⊤ {{ λ v, (@interp Σ) k τ HC Δ v }}.
+  Proof.
+    revert Hctx HC HΔ vs.
+    induction Htyped; intros Hctx HC HΔ vs Hlen; cbn.
+    - (* var *)
+      destruct (lookup_lt_is_Some_2 vs x) as [v Hv].
+      { by rewrite -Hlen; apply lookup_lt_Some with τ. }
+      rewrite /env_subst Hv /= -wp_value; eauto using to_of_val.
+      edestruct (zipwith_Forall_lookup _ Hctx) as [Hτ' Hτ'eq]; eauto.
+      etransitivity.
+      apply big_and_elem_of, elem_of_list_lookup_2 with x.
+      rewrite lookup_zip_with; simplify_option_eq; trivial.
+      rewrite interp_closed_irrel; trivial.
+    - (* unit *) value_case.
+    - (* pair *)
+      smart_wp_bind (PairLCtx e2.[env_subst vs]) _ v; eauto.
+      (* weird!: and_alwaysstable is an instance but is not resolved! *)
+      smart_wp_bind (PairRCtx v) (and_persistent _ _ _ _) v'.
+      value_case; eauto 10 with itauto.
+    - (* fst *)
+      smart_wp_bind (FstCtx) v. ipropsimpl; eauto.
+      apply const_elim_l; intros H; rewrite H.
+      rewrite -wp_fst; eauto using to_of_val, and_elim_l.
+      rewrite and_elim_l; rewrite interp_closed_irrel; eauto.
+    - (* snd *)
+      smart_wp_bind SndCtx v. ipropsimpl; eauto.
+      apply const_elim_l; intros H; rewrite H.
+      rewrite -wp_snd; eauto using to_of_val, and_elim_l.
+      rewrite and_elim_r; rewrite interp_closed_irrel; eauto.
+    - (* injl *) smart_wp_bind InjLCtx v; value_case; eauto 7 with itauto.
+    - (* injr *) smart_wp_bind InjRCtx v; value_case; eauto 7 with itauto.
+    - (* case *)
+      smart_wp_bind (CaseCtx _ _) _ v. cbn.
+      rewrite (later_intro (Π∧ zip_with
+           (λ (τ : {τ : type | closed_type k τ}) (v0 : leibniz_val),
+            ((interp k (` τ) (proj2_sig τ)) Δ) v0) (closed_ctx_list k Γ Hctx) vs));
+        rewrite or_elim; [apply impl_elim_l| |].
+      + rewrite exist_elim; eauto; intros v'.
+        apply const_elim_l; intros H; rewrite H.
+        rewrite -impl_intro_r //; rewrite -later_and later_mono; eauto.
+        rewrite -wp_case_inl; eauto using to_of_val.
+        asimpl.
+        specialize (IHHtyped2 Δ (typed_closed_ctx _ _ _ _ Htyped2) HC HΔ (v'::vs)).
+        erewrite <- ?typed_subst_head_simpl in * by (cbn; eauto).
+        rewrite -IHHtyped2; cbn; auto.
+        rewrite interp_closed_irrel type_context_closed_irrel /closed_ctx_list.
+        apply later_mono, and_intro; eauto 3 with itauto.
+      + rewrite exist_elim; eauto; intros v'.
+        apply const_elim_l; intros H; rewrite H.
+        rewrite -impl_intro_r //; rewrite -later_and later_mono; eauto.
+        rewrite -wp_case_inr; eauto using to_of_val.
+        asimpl.
+        specialize (IHHtyped3 Δ (typed_closed_ctx _ _ _ _ Htyped3) HC HΔ (v'::vs)).
+        erewrite <- ?typed_subst_head_simpl in * by (cbn; eauto).
+        rewrite -IHHtyped3; cbn; auto.
+        rewrite interp_closed_irrel type_context_closed_irrel /closed_ctx_list.
+        apply later_mono, and_intro; eauto 3 with itauto.    
+    - (* lam *)
+      value_case; apply (always_intro _ _), forall_intro=> v /=; apply impl_intro_l.
+      rewrite -wp_lam ?to_of_val //=.
+      asimpl. erewrite typed_subst_head_simpl; [|eauto|cbn]; eauto.
+      rewrite (later_intro (Π∧ _)) -later_and; apply later_mono.
+      rewrite interp_closed_irrel type_context_closed_irrel /closed_ctx_list.
+      rewrite -(IHHtyped Δ (typed_closed_ctx _ _ _ _ Htyped) (closed_type_arrow_2 HC) HΔ (v :: vs));
+        simpl; auto with f_equal.
+    - (* app *)
+      smart_wp_bind (AppLCtx (e2.[env_subst vs])) _ v.
+      rewrite -(@wp_bind _ _ _ [AppRCtx v]) /=.
+      rewrite -wp_impl_l /=; apply and_intro.
+      2: etransitivity; [|apply IHHtyped2]; eauto using and_elim_r.
+      rewrite and_elim_l. apply always_mono.
+      apply forall_intro =>v'.
+      rewrite forall_elim.
+      apply impl_intro_l.
+      rewrite -(later_intro).
+      etransitivity; [apply impl_elim_r|].
+      apply wp_mono => w.
+      rewrite interp_closed_irrel; trivial.
+    - (* TLam *)
+      value_case; rewrite -exist_intro; apply and_intro; auto.
+      apply forall_intro =>τi;
+        apply (always_intro _ _).
+      rewrite map_length in IHHtyped.
+      destruct τi as [τi τiAS].
+      specialize (IHHtyped
+                    (Vlist_cons τi Δ)
+                    (closed_ctx_map
+                       _ _ _ _
+                       Hctx (λ τ, closed_type_S_ren2 τ 1 0 _))
+                    (closed_type_forall HC)
+                    (alwyas_stable_Vlist_cons _ _ _ τiAS)
+                    _
+                    Hlen
+                 ).
+      rewrite -wp_impl_l -later_intro. apply and_intro;
+        [ apply (always_intro _ _), forall_intro=> v /=; apply impl_intro_l|].
+      2: etransitivity; [|apply IHHtyped].
+      + rewrite and_elim_l; trivial.
+      + rewrite zip_with_closed_ctx_list_subst; trivial.
+    - (* TApp *)
+      smart_wp_bind TAppCtx _ v; cbn.
+      rewrite and_elim_l.
+      rewrite exist_elim; eauto => e'.
+      apply const_elim_l; intros H'; rewrite H'.
+      rewrite (forall_elim ((interp k τ' H Δ) ↾ _)).
+      rewrite always_elim.
+      rewrite -wp_TLam; apply later_mono.
+      apply wp_mono=> w.
+      rewrite interp_subst; trivial.
+    - (* Fold *)
+      value_case. unfold interp_rec.
+      rewrite fixpoint_unfold.
+      cbn.
+      rewrite -exist_intro.
+      apply (always_intro _ _).
+      apply and_intro; auto.
+      rewrite map_length in IHHtyped.
+      specialize (IHHtyped
+                    (Vlist_cons (interp k (TRec τ) HC Δ) Δ)
+                    (closed_ctx_map
+                       _ _ _ _
+                       Hctx (λ τ, closed_type_S_ren2 τ 1 0 _))
+                    (closed_type_rec HC)
+                    (alwyas_stable_Vlist_cons _ _ _ _)
+                   _
+                    Hlen
+                 ).      
+      rewrite -wp_impl_l -later_intro. apply and_intro;
+        [ apply (always_intro _ _), forall_intro=> v /=; apply impl_intro_l|].
+      2: etransitivity; [|apply IHHtyped].
+      + rewrite and_elim_l; trivial.
+      + rewrite zip_with_closed_ctx_list_subst; trivial.
+    - (* Unfold *)
+      smart_wp_bind UnfoldCtx _ v; cbn.
+      rewrite and_elim_l.
+      unfold interp_rec. rewrite fixpoint_unfold /interp_rec_pre; cbn.
+      replace (fixpoint
+                 (λ rec_apr : leibniz_val -n> iProp lang Σ,
+                              CofeMor
+                                (λ w : leibniz_val,
+                                       □ (∃ e1 : expr,
+                                             w = FoldV e1
+                                             ∧ ▷ WP e1 @ ⊤ {{ λ v1 : val,
+                                                        ((interp (S k) τ (closed_type_rec ?HC4))
+                                                           (Vlist_cons rec_apr Δ)) v1 }}))%I))
+      with
+      (interp k (TRec τ) (typed_closed_type _ _ _ _ Htyped) Δ) by (cbn; unfold interp_rec; trivial).
+      rewrite always_elim.
+      rewrite exist_elim; eauto => e'.
+      apply const_elim_l; intros H'; rewrite H'.
+      rewrite -wp_Fold.
+      apply later_mono, wp_mono => w.
+      rewrite -interp_subst; eauto.
+      (* unshelving *)
+      Unshelve.
+      all: solve [eauto 2 using typed_closed_type | try typeclasses eauto].
+  Qed.
+  
+End typed_interp.
