prelude/base.v
@@ -1,0 +1,5 @@
+From mathcomp Require Export ssreflect.
+From iris.prelude Require Export prelude.
+Global Set Bullet Behavior "Strict Subproofs".
+Global Open Scope general_if_scope.
+Ltac done := prelude.tactics.done.
